rocq-osiris/stdlib/Stdlib.v
@@ -2,10 +2,14 @@
 (* From iris.bi Require Import weakestpre. *)
 (* From iris Require Import base_logic.lib.gen_heap. *)
 
-From osiris Require Import osiris.
+From osiris.lang Require Import lang.
+From osiris.semantics Require Import semantics.
 From osiris.logic Require Import orders.
-From osiris.stdlib Require Import Externals.
+From osiris Require Export Externals.
 From osiris.program_logic Require Import program_logic.
+From osiris.proofmode Require Import proofmode.
+
+Open Scope Z_scope.
 
 Local Transparent encode.
 
