rocq-osiris/theories/osiris.v
@@ -3,3 +3,4 @@ From osiris.lang Require Export lang.
 From osiris.semantics Require Export semantics.
 From osiris.program_logic Require Export program_logic.
 From osiris.proofmode Require Export proofmode.
+From osiris Require Export Stdlib.
